src/Expr.v
@@ -2,7 +2,7 @@ Require Import List DepList.
 Require Import EqdepClass.
 Require Import IL Word.
 Require Import Bool Folds.
-Require Import Reflection. 
+Require Import Reflection Tactics. 
 
 Set Implicit Arguments.
 
@@ -814,56 +814,64 @@ Section env.
     apply impl_to_semireflect; exact expr_seq_dec_correct.
   Qed.
 
-  (** lift the "real" variables in the range [a,...)
-   ** to the range [a+b,...)
-   **)
-  Fixpoint liftExpr (a b : nat) (e : expr) : expr :=
-    match e with
-      | Const t' c => Const t' c
-      | Var x => 
-        if NPeano.ltb x a
-        then Var x
-        else Var (x + b)
-      | UVar x => UVar x
-      | Func f xs => 
-        Func f (map (liftExpr a b) xs)
-      | Equal t e1 e2 => Equal t (liftExpr a b e1) (liftExpr a b e2)
-      | Not e1 => Not (liftExpr a b e1)
-    end.
+  Section liftExpr.
+    Variables ua ub : nat.
+    Variables a b : nat.
 
-  Fixpoint liftExprU (a b : nat) (e : expr (*(uvars' ++ uvars) vars*)) 
-    : expr (*(uvars' ++ ext ++ uvars) vars*) :=
-    match e with
-      | UVar x => 
-        if NPeano.ltb a x
-        then UVar x
-        else UVar (x + b)
-      | Var v => Var v
-      | Const t x => Const t x 
-      | Func f xs => 
-        Func f (map (liftExprU a b) xs)
-      | Equal t e1 e2 => Equal t (liftExprU a b e1) (liftExprU a b e2)
-      | Not e1 => Not (liftExprU a b e1)
-    end.
+    (** insert into the domain of e:
+     ** exprD (U ++ U') (G ++ G') e t = 
+     ** exprD (U ++ U'' ++ U') (G ++ G'' ++ G') (liftExpr (length U) (length U'') (length G) (length G'') e) t
+     **)
+    Fixpoint liftExpr (e : expr) : expr :=
+      match e with
+        | Const _ _ => e
+        | Var x => 
+          Var (if NPeano.ltb x a then x else b + x)
+        | UVar x => 
+          UVar (if NPeano.ltb x ua then x else ub + x)
+        | Func f xs => 
+          Func f (map liftExpr xs)
+        | Equal t e1 e2 => Equal t (liftExpr e1) (liftExpr e2)
+        | Not e1 => Not (liftExpr e1)
+      end.
+
+    Lemma liftExpr_0 : ub = 0 -> b = 0 -> forall e, liftExpr e = e.
+    Proof.
+      induction e; simpl; intros; think; simpl; auto;
+        try match goal with 
+              | [ |- context [ if ?X then _ else _ ] ] => destruct X
+            end; auto.
+      f_equal. induction H1; simpl in *; think; auto.
+    Qed.
+  End liftExpr.
+
+  Lemma liftExpr_combine : forall ua ub uc a b c e,
+    liftExpr ua ub a b (liftExpr ua uc a c e) = liftExpr ua (uc + ub) a (c + b) e.
+  Proof.
+    induction e; simpl; intros; think; auto; f_equal; unfold var, uvar in *;
+      repeat match goal with
+               | [ |- context [ if ?X then _ else _ ] ] => consider X; intros
+             end; try solve [ reflexivity | omega ].
+    induction H; intros; simpl; think; auto.
+  Qed.            
 
   (** This function replaces "real" variables [a, b) with existential variables (c,...)
-   ** TODO: the "b" parameter isn't really used!
    **)
   Fixpoint exprSubstU (a b c : nat) (s : expr (*a (b ++ c ++ d)*)) {struct s}
-      : expr (* (c ++ a) (b ++ d) *) :=
-      match s with
-        | Const _ t => Const _ t
-        | Var x =>
-          if NPeano.ltb x a 
-          then Var x
-          else if NPeano.ltb x b
-               then UVar (c + x - a)
-               else Var (x + a - b)
-        | UVar x => UVar x
-        | Func f args => Func f (map (exprSubstU a b c) args)
-        | Equal t e1 e2 => Equal t (exprSubstU a b c e1) (exprSubstU a b c e2)
-        | Not e1 => Not (exprSubstU a b c e1)
-      end.
+    : expr (* (c ++ a) (b ++ d) *) :=
+    match s with
+      | Const _ t => Const _ t
+      | Var x =>
+        if NPeano.ltb x a 
+        then Var x
+        else if NPeano.ltb x b
+             then UVar (c + x - a)
+             else Var (x + a - b)
+      | UVar x => UVar x
+      | Func f args => Func f (map (exprSubstU a b c) args)
+      | Equal t e1 e2 => Equal t (exprSubstU a b c e1) (exprSubstU a b c e2)
+      | Not e1 => Not (exprSubstU a b c e1)
+    end.
 
   Lemma nth_error_length : forall T (ls ls' : list T) n,
     nth_error (ls ++ ls') (n + length ls) = nth_error ls' n.
@@ -873,29 +881,6 @@ Section env.
     cutrewrite (n + S (length ls) = S n + length ls); [ | omega ]. simpl. auto.
   Qed.
 
-  Lemma liftExpr_0 : forall a (b : expr), liftExpr a 0 b = b.
-  Proof.
-    induction b; simpl; intros; auto.
-    destruct (NPeano.ltb x a); f_equal; omega.
-    f_equal. generalize dependent H. clear. induction 1. auto.
-    simpl; f_equal; auto.
-    rewrite IHb1; rewrite IHb2. reflexivity.
-    f_equal. auto.
-  Qed.
-
-  Lemma liftExpr_combine : forall (e : expr) a b c,
-    liftExpr a b (liftExpr a c e) = liftExpr a (c + b) e.
-  Proof.
-    induction e; intros; simpl; repeat match goal with
-                                         | [ H : _ |- _ ] => rewrite H
-                                       end; try reflexivity. 
-    consider (NPeano.ltb x a); simpl.
-    consider (NPeano.ltb x a); auto. intros; exfalso; omega.
-    consider (NPeano.ltb (x + c) a). intros; exfalso; omega. intros; f_equal; omega.
-    
-    f_equal. rewrite map_map. induction H; simpl; auto.
-    rewrite H. f_equal; auto.
-  Qed.            
 
   (** first variable in the list is the first one quantified
    **)
@@ -1102,59 +1087,45 @@ Proof.
   induction P; auto; intros; simpl in *; intuition eauto using Provable_weaken.
 Qed.
 
-Lemma liftExpr_ext : forall types (funcs : functions types) EG G G' G'' e t,
-  exprD funcs EG (G'' ++ G) e t = exprD funcs EG (G'' ++ G' ++ G) (liftExpr (length G'') (length G') e) t.
+Lemma nth_error_app_L : forall T (A B : list T) n,
+  (n < length A)%nat ->
+  nth_error (A ++ B) n = nth_error A n.
 Proof.
-  clear. induction e; simpl; intros; try reflexivity.
-  consider (NPeano.ltb x (length G'')); intros Hx. 
-  simpl. unfold lookupAs. 
-  revert G; revert G'. generalize dependent x. generalize dependent G''.
-  induction G''; simpl; intros.
-  exfalso; omega.
-  destruct x. reflexivity. simpl. erewrite <- IHG''. reflexivity. omega.
-  simpl. unfold lookupAs. 
+  induction A; destruct n; simpl; intros; try omega; auto.
+  eapply IHA. omega.
+Qed.
 
-  cutrewrite (x = (x - length G'') + length G''). 
-  cutrewrite ((x - length G'') + length G'' + length G' = (x - length G'') + length G' + length G''). 2: omega.
-  repeat rewrite nth_error_length. reflexivity.
-  rewrite Plus.plus_comm. rewrite <- Minus.le_plus_minus; auto. 
+Lemma nth_error_app_R : forall T (A B : list T) n,
+  (length A <= n)%nat ->
+  nth_error (A ++ B) n = nth_error B (n - length A).
+Proof.
+  induction A; destruct n; simpl; intros; try omega; auto.
+  apply IHA. omega. 
+Qed.
 
-  destruct (nth_error funcs f); auto. destruct (equiv_dec (Range s) t); auto.
-  unfold Equivalence.equiv in e. subst. destruct s; simpl in *.
-  generalize dependent Domain0. induction H; intros; auto.
-  simpl. destruct Domain0; auto. rewrite H.
-  match goal with
-    | [ |- match ?X with
-             | Some _ => _ | None => _ 
-           end _ _ = _ ] => destruct X
-  end. eauto.
 
-  auto.
-
-  destruct t0; auto. rewrite IHe1. rewrite IHe2. auto.
-
-  destruct t; auto. rewrite IHe. reflexivity.
+Lemma liftExpr_ext : forall types (funcs : functions types) U U' U'' G G' G'' e t,
+  exprD funcs (U'' ++ U) (G'' ++ G) e t =
+  exprD funcs (U'' ++ U' ++ U) (G'' ++ G' ++ G) (liftExpr (length U'') (length U') (length G'') (length G') e) t.
+Proof.
+  clear. induction e; simpl; intros; unfold lookupAs; think; try reflexivity;
+    repeat match goal with
+             | [ |- context [ NPeano.ltb ?X ?Y ] ] =>
+               consider (NPeano.ltb X Y); intros
+             | [ |- _ ] => rewrite nth_error_app_L by omega
+             | [ |- _ ] => rewrite nth_error_app_R by omega
+             | [ |- match nth_error _ ?X with _ => _ end = match nth_error _ ?Y with _ => _ end ] =>
+               cutrewrite (X = Y); try (reflexivity || omega)
+           end; auto.
+  destruct (nth_error funcs f); auto. destruct (equiv_dec (Range s) t); auto. unfold equiv in *. subst.
+    destruct s; simpl. generalize dependent Domain0; induction H; destruct Domain0; simpl; intros; think; auto.
+    destruct (exprD funcs (U'' ++ U' ++ U) (G'' ++ G' ++ G)
+       (liftExpr (length U'') (length U') (length G'') (length G') x) t); think; auto.
 Qed.
 
 Section exists_subst.
   Variable types : list type.
   Variable funcs : functions types.
-
-  Lemma nth_error_app_L : forall T (A B : list T) n,
-    (n < length A)%nat ->
-    nth_error (A ++ B) n = nth_error A n.
-  Proof.
-    induction A; destruct n; simpl; intros; try omega; auto.
-    eapply IHA. omega.
-  Qed.
-
-  Lemma nth_error_app_R : forall T (A B : list T) n,
-    (length A <= n)%nat ->
-    nth_error (A ++ B) n = nth_error B (n - length A).
-  Proof.
-    induction A; destruct n; simpl; intros; try omega; auto.
-    apply IHA. omega. 
-  Qed.
 
   Theorem exprSubstU_spec : forall e a b c e',
     exprSubstU a b c e = e' ->
