examples/AutoSep.v
@@ -181,7 +181,7 @@ Ltac hints_ext_simplifier hints := fun s1 s2 s3 H =>
          Expr.tvar_val_seqb_correct
          Expr.tvar_seqb_correct
          Expr.ReifyExpr.default_type
-
+         Expr.mentionsU
 
          (** ExprUnify **)
          U.exprUnify U.exprUnify_recursor
@@ -190,7 +190,7 @@ Ltac hints_ext_simplifier hints := fun s1 s2 s3 H =>
          U.Subst_empty U.subst_empty
          U.Subst_set U.subst_set
          U.Subst_equations
-         U.mentionsU
+         U.Subst_size
          U.dep_in
          U.exprUnify_recursor
 
@@ -225,6 +225,7 @@ Ltac hints_ext_simplifier hints := fun s1 s2 s3 H =>
          Unfolder.allb UNF.substExpr UNF.substSheap
          UNF.find UNF.default_hintsPayload
          UNF.substExprBw UNF.substExprBw' UNF.substSheapBw
+         UNF.applicable UNF.checkAllInstantiated
 
          (** NatMap **)
          NatMap.singleton
@@ -339,11 +340,11 @@ Ltac hints_ext_simplifier hints := fun s1 s2 s3 H =>
          SEP.Default_predicate
          SEP.himp SEP.sexprD
          SEP.heq
+         SEP.liftSExpr
 
          (** SepHeap **)
          SH.impures SH.pures SH.other
          SH.liftSHeap SH.sheapSubstU
-         SH.sheap_liftVars
          SH.starred SH.hash 
          SH.star_SHeap 
          SH.SHeap_empty 
@@ -475,6 +476,7 @@ Ltac hints_ext_simplifier hints := fun s1 s2 s3 H =>
          Expr.tvar_val_seqb_correct
          Expr.tvar_seqb_correct
          Expr.ReifyExpr.default_type
+         Expr.mentionsU
 
          (** ExprUnify **)
          U.exprUnify U.exprUnify_recursor
@@ -483,7 +485,7 @@ Ltac hints_ext_simplifier hints := fun s1 s2 s3 H =>
          U.Subst_empty U.subst_empty
          U.Subst_set U.subst_set
          U.Subst_equations
-         U.mentionsU
+         U.Subst_size
          U.dep_in
          U.exprUnify_recursor
 
@@ -517,6 +519,7 @@ Ltac hints_ext_simplifier hints := fun s1 s2 s3 H =>
          Unfolder.allb UNF.substExpr UNF.substSheap
          UNF.find UNF.default_hintsPayload
          UNF.substExprBw UNF.substExprBw' UNF.substSheapBw
+         UNF.applicable UNF.checkAllInstantiated
 
          (** NatMap **)
          NatMap.singleton
@@ -635,11 +638,11 @@ Ltac hints_ext_simplifier hints := fun s1 s2 s3 H =>
          SEP.himp SEP.sexprD
          SEP.heq
          nat_eq_eqdec
+         SEP.liftSExpr
 
          (** SepHeap **)
          SH.impures SH.pures SH.other
          SH.liftSHeap SH.sheapSubstU
-         SH.sheap_liftVars
          SH.starred SH.hash 
          SH.star_SHeap 
          SH.SHeap_empty 
@@ -779,7 +782,7 @@ Ltac sepLemma := unfold Himp in *; simpl; intros; cancel auto_ext.
 (** env -> fwd -> bwd -> (hints -> T) -> T **)
 Ltac prepare := 
   let the_unfold_tac x := 
-    eval unfold empB injB injBX starB exB hvarB in x
+    eval unfold empB, injB, injBX, starB, exB, hvarB in x
   in
   SymILTac.PACKAGED.prepareHints the_unfold_tac W (settings * state)%type isConst.
 
